feat(library/init/data/array): store dimension in the array
The array dimension is now stored inside the array.
The main motivation is that it reflects the actual runtime implementation.
We need to store the array size to be able to GC it.
So, it feels silly to have the array size stored in each array object,
but we cannot use this information.
For example, in the `hashmap` we implemented the bucket array using
`array`, and we store the `size` of the array.
Same for the Lean3 `buffer` object.
The `buffer` object doesn't even need to exist.
The actual `array` implementation is the `buffer`

src/library/vm/vm_array.cpp
@@ -63,16 +63,20 @@ vm_obj to_obj(parray<vm_obj> const & a) {
     return mk_vm_external(new vm_array(a));
 }
 
-vm_obj d_array_read(vm_obj const &, vm_obj const &, vm_obj const & a, vm_obj const & i) {
-    /* TODO(Leo): handle case where n is too big */
+vm_obj array_sz(vm_obj const &, vm_obj const & a) {
+    return mk_vm_nat(to_array(a).size());
+}
+
+vm_obj array_read(vm_obj const &, vm_obj const & a, vm_obj const & i) {
+    /* TODO(Leo): handle case where i is too big */
     unsigned idx = force_to_unsigned(i);
     lean_vm_check(idx < to_array(a).size());
     parray<vm_obj> const & _a = to_array(a);
     return _a[idx];
 }
 
-vm_obj d_array_write(vm_obj const &, vm_obj const &, vm_obj const & a, vm_obj const & i, vm_obj const & v) {
-    /* TODO(Leo): handle case where n is too big */
+vm_obj array_write(vm_obj const &, vm_obj const & a, vm_obj const & i, vm_obj const & v) {
+    /* TODO(Leo): handle case where i is too big */
     unsigned idx = force_to_unsigned(i);
     parray<vm_obj> const & p = to_array(a);
     lean_vm_check(idx < p.size());
@@ -86,7 +90,7 @@ vm_obj d_array_write(vm_obj const &, vm_obj const &, vm_obj const & a, vm_obj co
     }
 }
 
-vm_obj array_push_back(vm_obj const &, vm_obj const &, vm_obj const & a, vm_obj const & v) {
+vm_obj array_push(vm_obj const &, vm_obj const & a, vm_obj const & v) {
     parray<vm_obj> const & p = to_array(a);
     if (a.raw()->get_rc() == 1) {
         const_cast<parray<vm_obj> &>(p).push_back(v);
@@ -98,7 +102,7 @@ vm_obj array_push_back(vm_obj const &, vm_obj const &, vm_obj const & a, vm_obj 
     }
 }
 
-vm_obj array_pop_back(vm_obj const &, vm_obj const &, vm_obj const & a) {
+vm_obj array_pop(vm_obj const &, vm_obj const & a) {
     parray<vm_obj> const & p = to_array(a);
     if (a.raw()->get_rc() == 1) {
         const_cast<parray<vm_obj> &>(p).pop_back();
@@ -117,7 +121,7 @@ vm_obj mk_array(vm_obj const & /* alpha */, vm_obj const & n, vm_obj const & v) 
     return to_obj(a);
 }
 
-vm_obj d_array_mk(vm_obj const & n, vm_obj const & /* alpha */, vm_obj const & fn) {
+vm_obj array_mk(vm_obj const & /* alpha */, vm_obj const & n, vm_obj const & fn) {
     /* TODO(Leo): handle case where n is too big */
     unsigned _n = force_to_unsigned(n);
     parray<vm_obj> a;
@@ -127,10 +131,10 @@ vm_obj d_array_mk(vm_obj const & n, vm_obj const & /* alpha */, vm_obj const & f
     return to_obj(a);
 }
 
-vm_obj d_array_foreach(vm_obj const & n, vm_obj const & /* alpha */, vm_obj const & a, vm_obj const & fn) {
+vm_obj array_foreach(vm_obj const & /* alpha */, vm_obj const & a, vm_obj const & fn) {
     /* TODO(Leo): handle case where n is too big */
-    unsigned _n = force_to_unsigned(n);
     parray<vm_obj> const & p = to_array(a);
+    unsigned _n = p.size();
     if (a.raw()->get_rc() == 1) {
         parray<vm_obj> & _p = const_cast<parray<vm_obj> &>(p);
         for (unsigned i = 0; i < _n; i++)
@@ -145,11 +149,10 @@ vm_obj d_array_foreach(vm_obj const & n, vm_obj const & /* alpha */, vm_obj cons
     }
 }
 
-vm_obj d_array_iterate(vm_obj const & n, vm_obj const & /* alpha */, vm_obj const & /* beta */,
-                       vm_obj const & a, vm_obj const & b, vm_obj const & fn) {
-    /* TODO(Leo): handle case where n is too big */
-    unsigned _n = force_to_unsigned(n);
+vm_obj array_iterate(vm_obj const & /* alpha */, vm_obj const & /* beta */,
+                     vm_obj const & a, vm_obj const & b, vm_obj const & fn) {
     parray<vm_obj> const & p = to_array(a);
+    unsigned _n              = p.size();
     vm_obj r = b;
     for (unsigned i = 0; i < _n; i++)
         r = invoke(fn, mk_vm_nat(i), p[i], r);
@@ -158,30 +161,32 @@ vm_obj d_array_iterate(vm_obj const & n, vm_obj const & /* alpha */, vm_obj cons
 
 static unsigned g_array_read_idx = -1;
 
-unsigned d_array_cases_on(vm_obj const & o, buffer<vm_obj> & data) {
-    vm_obj d[3] = {o, mk_vm_unit(), mk_vm_unit()};
-    vm_obj fn = mk_vm_closure(g_array_read_idx, 3, d);
+unsigned array_cases_on(vm_obj const & o, buffer<vm_obj> & data) {
+    vm_obj d[2] = {o, mk_vm_unit()};
+    vm_obj fn = mk_vm_closure(g_array_read_idx, 2, d);
+    data.push_back(mk_vm_nat(to_array(o).size()));
     data.push_back(fn);
     return 0;
 }
 
 void initialize_vm_array() {
-    DECLARE_VM_BUILTIN(name({"d_array", "mk"}),             d_array_mk);
-    DECLARE_VM_BUILTIN(name({"mk_array"}),                  mk_array);
-    DECLARE_VM_BUILTIN(name({"d_array", "data"}),           d_array_read);
-    DECLARE_VM_BUILTIN(name({"d_array", "read"}),           d_array_read);
-    DECLARE_VM_BUILTIN(name({"d_array", "write"}),          d_array_write);
-    DECLARE_VM_BUILTIN(name({"array", "push_back"}),        array_push_back);
-    DECLARE_VM_BUILTIN(name({"array", "pop_back"}),         array_pop_back);
-    DECLARE_VM_BUILTIN(name({"d_array", "foreach"}),        d_array_foreach);
-    DECLARE_VM_BUILTIN(name({"d_array", "iterate"}),        d_array_iterate);
-    DECLARE_VM_CASES_BUILTIN(name({"d_array", "cases_on"}), d_array_cases_on);
+    DECLARE_VM_BUILTIN(name({"array", "mk"}),             array_mk);
+    DECLARE_VM_BUILTIN(name({"mk_array"}),                mk_array);
+    DECLARE_VM_BUILTIN(name({"array", "sz"}),             array_sz);
+    DECLARE_VM_BUILTIN(name({"array", "data"}),           array_read);
+    DECLARE_VM_BUILTIN(name({"array", "read"}),           array_read);
+    DECLARE_VM_BUILTIN(name({"array", "write"}),          array_write);
+    DECLARE_VM_BUILTIN(name({"array", "push"}),           array_push);
+    DECLARE_VM_BUILTIN(name({"array", "pop"}),            array_pop);
+    DECLARE_VM_BUILTIN(name({"array", "foreach"}),        array_foreach);
+    DECLARE_VM_BUILTIN(name({"array", "iterate"}),        array_iterate);
+    DECLARE_VM_CASES_BUILTIN(name({"array", "cases_on"}), array_cases_on);
 }
 
 void finalize_vm_array() {
 }
 
 void initialize_vm_array_builtin_idxs() {
-    g_array_read_idx = *get_vm_builtin_idx(name({"d_array", "read"}));
+    g_array_read_idx = *get_vm_builtin_idx(name({"array", "read"}));
 }
 }
