tests/lean/run/array1.lean
@@ -1,0 +1,27 @@
+#check @array.mk
+
+#eval mk_array 4 1
+
+def v : array nat := @array.mk nat 10 (λ ⟨i, _⟩, i)
+
+#eval array.map (+10) v
+
+def w : array nat :=
+(mk_array 9 1).push 3
+
+def f : fin w.sz → nat :=
+array.cases_on w (λ _ f, f)
+
+#eval f ⟨1, sorry⟩
+#eval f ⟨9, sorry⟩
+
+#eval (((mk_array 1 1).push 2).push 3).foldl 0 (+)
+
+def array_sum (a : array nat) : nat :=
+a.foldl 0 (+)
+
+#eval array_sum (mk_array 10 1)
+
+#eval (mk_array 10 1).data ⟨1, dec_trivial⟩ + 20
+#eval (mk_array 10 1).data ⟨2, dec_trivial⟩
+#eval (mk_array 10 3).data ⟨2, dec_trivial⟩
